src/library/tactic/simplify.cpp
@@ -32,6 +32,7 @@ Author: Daniel Selsam, Leonardo de Moura
 #include "library/vm/vm_expr.h"
 #include "library/vm/vm_option.h"
 #include "library/vm/vm_list.h"
+#include "library/vm/vm_nat.h"
 #include "library/vm/vm_name.h"
 #include "library/tactic/tactic_state.h"
 #include "library/tactic/ac_tactics.h"
@@ -814,8 +815,40 @@ simp_result simplify_ext_core_fn::forall_congr(expr const & e) {
 }
 
 simp_result simplify_ext_core_fn::imp_congr(expr const & e) {
-    // TODO(Leo)
-    return simp_result(e);
+    expr const & a  = binding_domain(e);
+    expr const & b  = binding_body(e);
+    simp_result r_a = visit(a, some_expr(e));
+    if (m_contextual) {
+        type_context::tmp_locals locals(m_ctx);
+        expr h = locals.push_local("_h", r_a.get_new());
+        flet<simp_lemmas> set_slss(m_slss, add_to_slss(m_slss, locals.as_buffer()));
+        freset<simplify_cache> reset_cache(m_cache);
+        simp_result r_b = visit(b, some_expr(e));
+        if (r_a.get_new() == a && r_b.get_new() == b) {
+            return e;
+        } else if (!r_a.has_proof() && !r_b.has_proof()) {
+            return simp_result(mk_arrow(r_a.get_new(), r_b.get_new()));
+        } else {
+            expr fn   = mk_constant(m_rel == get_eq_name() ? get_imp_congr_ctx_eq_name() : get_imp_congr_ctx_name());
+            expr pr_a = finalize(m_ctx, m_rel, r_a).get_proof();
+            expr pr_b = locals.mk_lambda(finalize(m_ctx, m_rel, r_b).get_proof());
+            expr pr = mk_app({fn, a, b, r_a.get_new(), r_b.get_new(), pr_a, pr_b});
+            return simp_result(mk_arrow(r_a.get_new(), r_b.get_new()), pr);
+        }
+    } else {
+        simp_result r_b = visit(b, some_expr(e));
+        if (r_a.get_new() == a && r_b.get_new() == b) {
+            return e;
+        } else if (!r_a.has_proof() && !r_b.has_proof()) {
+            return simp_result(mk_arrow(r_a.get_new(), r_b.get_new()));
+        } else {
+            expr fn   = mk_constant(m_rel == get_eq_name() ? get_imp_congr_eq_name() : get_imp_congr_name());
+            expr pr_a = finalize(m_ctx, m_rel, r_a).get_proof();
+            expr pr_b = finalize(m_ctx, m_rel, r_b).get_proof();
+            expr pr = mk_app({fn, a, b, r_a.get_new(), r_b.get_new(), pr_a, pr_b});
+            return simp_result(mk_arrow(r_a.get_new(), r_b.get_new()), pr);
+        }
+    }
 }
 
 simp_result simplify_ext_core_fn::visit_pi(expr const & e) {
@@ -920,981 +953,115 @@ public:
                              canonize_instances, canonize_proofs, use_axioms),
         m_prove(prove), m_pre(pre), m_post(post),
         m_s(mk_tactic_state_for(ctx.env(), ctx.get_options(), ctx.mctx(), ctx.lctx(), mk_true())) {}
-};
 
-void initialize_new_simplify() {
-}
-
-void finalize_new_simplify() {
-}
-
-/* LEGACY */
-
-
-
-static name * g_simplify_prefix = nullptr;
-name get_simplify_prefix_name() { return *g_simplify_prefix; }
-
-/* Options */
-
-static name * g_simplify_max_steps                      = nullptr;
-static name * g_simplify_contextual                     = nullptr;
-static name * g_simplify_rewrite                        = nullptr;
-static name * g_simplify_lift_eq                        = nullptr;
-static name * g_simplify_canonize_instances_fixed_point = nullptr;
-static name * g_simplify_canonize_proofs_fixed_point    = nullptr;
-
-name get_simplify_max_steps_name() { return *g_simplify_max_steps; }
-name get_simplify_contextual_name() { return *g_simplify_contextual; }
-name get_simplify_rewrite_name() { return *g_simplify_rewrite; }
-name get_simplify_lift_eq_name() { return *g_simplify_lift_eq; }
-name get_simplify_canonize_instances_fixed_point_name() { return *g_simplify_canonize_instances_fixed_point; }
-name get_simplify_canonize_proofs_fixed_point_name() { return *g_simplify_canonize_proofs_fixed_point; }
-
-static unsigned get_simplify_max_steps(options const & o) {
-    return o.get_unsigned(*g_simplify_max_steps, LEAN_DEFAULT_SIMPLIFY_MAX_STEPS);
-}
-
-static bool get_simplify_contextual(options const & o) {
-    return o.get_bool(*g_simplify_contextual, LEAN_DEFAULT_SIMPLIFY_CONTEXTUAL);
-}
-
-static bool get_simplify_rewrite(options const & o) {
-    return o.get_bool(*g_simplify_rewrite, LEAN_DEFAULT_SIMPLIFY_REWRITE);
-}
-
-static bool get_simplify_lift_eq(options const & o) {
-    return o.get_bool(*g_simplify_lift_eq, LEAN_DEFAULT_SIMPLIFY_LIFT_EQ);
-}
-
-static bool get_simplify_canonize_instances_fixed_point(options const & o) {
-    return o.get_bool(*g_simplify_canonize_instances_fixed_point,
-                      LEAN_DEFAULT_SIMPLIFY_DEFEQ_CANONIZE_INSTANCES_FIXED_POINT);
-}
-
-static bool get_simplify_canonize_proofs_fixed_point(options const & o) {
-    return o.get_bool(*g_simplify_canonize_proofs_fixed_point, LEAN_DEFAULT_SIMPLIFY_DEFEQ_CANONIZE_PROOFS_FIXED_POINT);
-}
-
-/* Main simplifier class */
-
-class simplifier {
-    type_context              m_tctx, m_tctx_whnf;
-
-    name                      m_rel;
-
-    simp_lemmas               m_slss;
-
-    optional<vm_obj>          m_prove_fn;
-
-    /* Logging */
-    unsigned                  m_num_steps{0};
-
-    bool                      m_need_restart{false};
-
-    /* Options */
-    unsigned                  m_max_steps;
-    bool                      m_contextual;
-    bool                      m_rewrite;
-    bool                      m_lift_eq;
-    bool                      m_canonize_instances_fixed_point;
-    bool                      m_canonize_proofs_fixed_point;
-
-    typedef expr_struct_map<simp_result> simplify_cache;
-    simplify_cache m_cache;
-    optional<simp_result> cache_lookup(expr const & e);
-    void cache_save(expr const & e, simp_result const & r);
-
-    /* Basic helpers */
-    environment const & env() const { return m_tctx.env(); }
-
-    simp_result join(simp_result const & r1, simp_result const & r2) { return ::lean::join(m_tctx, m_rel, r1, r2); }
-
-    bool using_eq() { return m_rel == get_eq_name(); }
-
-    bool is_dependent_fn(expr const & f) {
-        expr f_type = m_tctx.whnf(m_tctx.infer(f));
-        lean_assert(is_pi(f_type));
-        return has_free_vars(binding_body(f_type));
-    }
-
-    simp_lemmas add_to_slss(simp_lemmas const & _slss, buffer<expr> const & ls) {
-        simp_lemmas slss = _slss;
-        for (unsigned i = 0; i < ls.size(); i++) {
-            expr const & l = ls[i];
-            try {
-                // TODO(Leo,Daniel): should we allow the user to set the priority of local lemmas?
-                slss = add(m_tctx, slss, mlocal_name(l), m_tctx.infer(l), l, LEAN_DEFAULT_PRIORITY);
-                lean_trace_d(name({"simplifier", "context"}), tout() << mlocal_name(l) << " : " << m_tctx.infer(l) << "\n";);
-            } catch (exception e) {
-            }
-        }
-        return slss;
-    }
-
-    bool should_defeq_canonize() {
-        return m_canonize_instances_fixed_point || m_canonize_proofs_fixed_point;
-    }
-
-    bool instantiate_emetas(tmp_type_context & tmp_tctx, unsigned num_emeta,
-                            list<expr> const & emetas, list<bool> const & instances);
-
-    /* Simp_Results */
-    simp_result lift_from_eq(expr const & old_e, simp_result const & r_eq);
-
-    /* Main simplify method */
-    simp_result simplify(expr const & old_e) {
-        m_num_steps++;
-        lean_trace_inc_depth("simplifier");
-        lean_trace_d("simplifier", tout() << m_rel << ": " << old_e << "\n";);
-
-        if (m_num_steps > m_max_steps) {
-            lean_trace(name({"simplifier", "failed"}), tout() << m_rel << ": " << old_e << "\n";);
-            throw exception("simplifier failed, maximum number of steps exceeded");
-        }
-
-        if (auto it = cache_lookup(old_e))
-            return *it;
-
-        expr e = whnf_eta(old_e);
-        simp_result r;
-
-        r = simplify_binary(e);
-
-        if (!r.is_done())
-            r = join(r, simplify(r.get_new()));
-
-        if (m_lift_eq && !using_eq()) {
-            simp_result r_eq;
-            {
-                flet<name> use_eq(m_rel, get_eq_name());
-                r_eq = simplify(r.get_new());
-            }
-            if (r_eq.get_new() != r.get_new()) {
-                r = join(r, lift_from_eq(r.get_new(), r_eq));
-                r = join(r, simplify(r.get_new()));
-            }
-        }
-
-        cache_save(old_e, r);
-
-        return r;
-    }
-
-    simp_result simplify_rewrite_binary(expr const & e) {
-        simp_lemmas_for const * sr = m_slss.find(m_rel);
-        if (!sr) return simp_result(e);
-
-        list<simp_lemma> const * srs = sr->find(e);
-        if (!srs) {
-            lean_trace_d(name({"debug", "simplifier", "try_rewrite"}), tout() << "no simp lemmas for: " << e << "\n";);
-            return simp_result(e);
-        }
-
-        for (simp_lemma const & lemma : *srs) {
-            simp_result r = rewrite_binary(e, lemma);
-            if (!is_eqp(r.get_new(), e)) {
-                lean_trace_d(name({"simplifier", "rewrite"}), tout() << "[" << lemma.get_id() << "]: " << e <<
-                             " ==> " << r.get_new() << "\n";);
-                return r;
-            }
-        }
-        return simp_result(e);
-    }
-
-    simp_result rewrite_binary(expr const & e, simp_lemma const & sl) {
-        tmp_type_context tmp_tctx(m_tctx, sl.get_num_umeta(), sl.get_num_emeta());
-        if (!tmp_tctx.is_def_eq(e, sl.get_lhs())) {
-            lean_trace_d(name({"debug", "simplifier", "try_rewrite"}), tout() << "fail to unify: " << sl.get_id() << "\n";);
-            return simp_result(e);
-        }
-        if (!instantiate_emetas(tmp_tctx, sl.get_num_emeta(), sl.get_emetas(), sl.get_instances())) {
-            lean_trace_d(name({"debug", "simplifier", "try_rewrite"}), tout() << "fail to instantiate emetas: " <<
-                         sl.get_id() << "\n";);
-            return simp_result(e);
-        }
-
-        for (unsigned i = 0; i < sl.get_num_umeta(); i++) {
-            if (!tmp_tctx.is_uassigned(i))
-                return simp_result(e);
-        }
-
-        expr new_lhs = tmp_tctx.instantiate_mvars(sl.get_lhs());
-        expr new_rhs = tmp_tctx.instantiate_mvars(sl.get_rhs());
-        if (sl.is_permutation()) {
-            if (!is_lt(new_rhs, new_lhs, false)) {
-                lean_simp_trace(tmp_tctx, name({"simplifier", "perm"}),
-                                tout() << "perm rejected: " << new_rhs << " !< " << new_lhs << "\n";);
-                return simp_result(e);
-            }
-        }
-
-        if (sl.is_refl()) {
-            return simp_result(new_rhs);
-        } else {
-            expr pf = tmp_tctx.instantiate_mvars(sl.get_proof());
-            return simp_result(new_rhs, pf);
-        }
-    }
-
-    simp_result simplify_subterms_app_binary(expr const & _e) {
-        lean_assert(is_app(_e));
-        expr e = should_defeq_canonize() ? defeq_canonize_args_step(_e) : _e;
-
-        // (1) Try user-defined congruences
-        simp_result r_user = try_congrs(e);
-        if (r_user.has_proof()) {
-            if (using_eq()) {
-                return join(r_user, simplify_operator_of_app(r_user.get_new()));
-            } else {
-                return r_user;
-            }
-        }
-
-        // (2) Synthesize congruence lemma
-        if (using_eq()) {
-            optional<simp_result> r_args = synth_congr(e);
-            if (r_args) return join(*r_args, simplify_operator_of_app(r_args->get_new()));
-        }
-        // (3) Fall back on generic binary congruence
-        if (using_eq()) {
-            expr const & f = app_fn(e);
-            expr const & arg = app_arg(e);
-
-            simp_result r_f = simplify(f);
-
-            if (is_dependent_fn(f)) {
-                if (r_f.has_proof()) return congr_fun(r_f, arg);
-                else return mk_app(r_f.get_new(), arg);
-            } else {
-                simp_result r_arg = simplify(arg);
-                return congr_fun_arg(r_f, r_arg);
-            }
-        }
-        return simp_result(e);
-    }
-
-
-    // Main binary simplify method
-    simp_result simplify_binary(expr const & e) {
-        // [1] Simplify subterms using congruence
-        simp_result r(e);
-
-        switch (r.get_new().kind()) {
-        case expr_kind::Local:
-        case expr_kind::Meta:
-        case expr_kind::Sort:
-        case expr_kind::Constant:
-        case expr_kind::Macro:
-            // no-op
-            break;
-        case expr_kind::Lambda:
-            if (using_eq())
-                r = simplify_subterms_lambda(r.get_new());
-            break;
-        case expr_kind::Pi:
-            r = simplify_subterms_pi(r.get_new());
-            break;
-        case expr_kind::App:
-            r = simplify_subterms_app_binary(r.get_new());
-            break;
-        case expr_kind::Let:
-            // whnf unfolds let-expressions
-            // TODO(dhs, leo): add flag for type_context not to unfold let-expressions
-            lean_unreachable();
-        case expr_kind::Var:
-            lean_unreachable();
-        }
-
-        if (r.get_new() != e) {
-            lean_trace_d(name({"simplifier", "congruence"}), tout() << e << " ==> " << r.get_new() << "\n";);
-        }
-
-        if (m_rewrite) {
-            simp_result r_rewrite = simplify_rewrite_binary(r.get_new());
-            if (r_rewrite.get_new() != r.get_new()) {
-                lean_trace_d(name({"simplifier", "rewrite"}), tout() << r.get_new() << " ==> " <<
-                             r_rewrite.get_new() << "\n";);
-                return join(r, r_rewrite);
-            }
-        }
-
-        r.set_done();
-        return r;
-    }
-
-    /* Simplifying the necessary subterms */
-    simp_result simplify_subterms_lambda(expr const & e);
-    simp_result simplify_subterms_pi(expr const & e);
-    simp_result simplify_subterms_app(expr const & e);
-
-    /* Called from simplify_subterms_app */
-    simp_result simplify_operator_of_app(expr const & e);
-
-    /* Proving */
-    optional<expr> prove(expr const & thm);
-
-    /* Canonize */
-    expr defeq_canonize_args_step(expr const & e);
-
-    /* Congruence */
-    simp_result congr_fun_arg(simp_result const & r_f, simp_result const & r_arg);
-    simp_result congr(simp_result const & r_f, simp_result const & r_arg);
-    simp_result congr_fun(simp_result const & r_f, expr const & arg);
-    simp_result congr_arg(expr const & f, simp_result const & r_arg);
-    simp_result congr_funs(simp_result const & r_f, buffer<expr> const & args);
-    simp_result funext(simp_result const & r, expr const & l);
-
-    simp_result try_congrs(expr const & e);
-    simp_result try_congr(expr const & e, simp_lemma const & cr);
-
-    optional<simp_result> synth_congr(expr const & e);
-
-    expr remove_unnecessary_casts(expr const & e);
-
-    /* Apply whnf and eta-reduction
-       \remark We want (Sum n (fun x, f x)) and (Sum n f) to be the same.
-       \remark We may want to switch to eta-expansion later (see paper: "The Virtues of Eta-expansion").
-       TODO(Daniel, Leo): should we add an option for disabling/enabling eta? */
-    expr whnf_eta(expr const & e);
-
-public:
-    simplifier(type_context & tctx, type_context & tctx_whnf, name const & rel, simp_lemmas const & slss, optional<vm_obj> const & prove_fn):
-        m_tctx(tctx), m_tctx_whnf(tctx_whnf), m_rel(rel), m_slss(slss), m_prove_fn(prove_fn),
-        /* Options */
-        m_max_steps(get_simplify_max_steps(tctx.get_options())),
-        m_contextual(get_simplify_contextual(tctx.get_options())),
-        m_rewrite(get_simplify_rewrite(tctx.get_options())),
-        m_lift_eq(get_simplify_lift_eq(tctx.get_options())),
-        m_canonize_instances_fixed_point(get_simplify_canonize_instances_fixed_point(tctx.get_options())),
-        m_canonize_proofs_fixed_point(get_simplify_canonize_proofs_fixed_point(tctx.get_options()))
-        {}
-
-    simp_result operator()(expr const & e)  {
-        scope_trace_env scope(env(), m_tctx.get_options(), m_tctx);
-        simp_result r(e);
-        while (true) {
-            m_need_restart = false;
-            r = join(r, simplify(r.get_new()));
-            if (!m_need_restart || !should_defeq_canonize())
-                return r;
-            m_cache.clear();
-        }
-        return simplify(e);
+    pair<vm_obj, simp_result> operator()(vm_obj const & a, name const & rel, expr const & e) {
+        m_a = a;
+        auto r = simplify_ext_core_fn::operator()(rel, e);
+        return mk_pair(m_a, r);
     }
 };
 
-/* Cache */
-
-optional<simp_result> simplifier::cache_lookup(expr const & e) {
-    auto it = m_cache.find(e);
-    if (it == m_cache.end()) return optional<simp_result>();
-    return optional<simp_result>(it->second);
+/*
+structure simplify_config :=
+(max_steps : nat)
+(contextual : bool)
+(lift_eq : bool)
+(canonize_instances : bool)
+(canonize_proofs : bool)
+(use_axioms : bool)
+*/
+void get_simplify_config(vm_obj const & obj, unsigned & max_steps, bool & contextual, bool & lift_eq,
+                         bool & canonize_instances, bool & canonize_proofs, bool & use_axioms) {
+    max_steps          = force_to_unsigned(cfield(obj, 0), std::numeric_limits<unsigned>::max());
+    contextual         = to_bool(cfield(obj, 1));
+    lift_eq            = to_bool(cfield(obj, 2));
+    canonize_instances = to_bool(cfield(obj, 3));
+    canonize_proofs    = to_bool(cfield(obj, 4));
+    use_axioms         = to_bool(cfield(obj, 5));
 }
 
-void simplifier::cache_save(expr const & e, simp_result const & r) {
-    m_cache.insert(mk_pair(e, r));
-}
-
-/* Simp_Results */
-
-simp_result simplifier::lift_from_eq(expr const & old_e, simp_result const & r_eq) {
-    if (!r_eq.has_proof()) return r_eq;
-    lean_assert(r_eq.has_proof());
-    /* r_eq.get_proof() : old_e = r_eq.get_new() */
-    /* goal : old_e <m_rel> r_eq.get_new() */
-    type_context::tmp_locals local_factory(m_tctx);
-    expr local = local_factory.push_local(name(), m_tctx.infer(old_e));
-    expr motive_local = mk_app(m_tctx, m_rel, old_e, local);
-    /* motive = fun y, old_e <m_rel> y */
-    expr motive = local_factory.mk_lambda(motive_local);
-    /* Rxx = x <m_rel> x */
-    expr Rxx = mk_refl(m_tctx, m_rel, old_e);
-    expr pf = mk_eq_rec(m_tctx, motive, Rxx, r_eq.get_proof());
-    return simp_result(r_eq.get_new(), pf);
-}
-
-/* Whnf + Eta */
-expr simplifier::whnf_eta(expr const & e) {
-    return try_eta(m_tctx_whnf.whnf(e));
-}
-
-simp_result simplifier::simplify_subterms_lambda(expr const & old_e) {
-    lean_assert(is_lambda(old_e));
-    expr e = old_e;
-
-    buffer<expr> ls;
-    while (is_lambda(e)) {
-        expr d = instantiate_rev(binding_domain(e), ls.size(), ls.data());
-        expr l = m_tctx.push_local(binding_name(e), d, binding_info(e));
-        ls.push_back(l);
-        e = instantiate(binding_body(e), l);
-    }
-
-    simp_result r = simplify(e);
-    expr new_e = r.get_new();
-
-    if (r.get_new() == e)
-        return old_e;
-
-    if (!r.has_proof())
-        return m_tctx.mk_lambda(ls, r.get_new());
-
-    for (int i = ls.size() - 1; i >= 0; --i)
-        r = funext(r, ls[i]);
-
-    return r;
-}
-
-simp_result simplifier::simplify_subterms_pi(expr const & e) {
-    lean_assert(is_pi(e));
-    return try_congrs(e);
-}
-
-expr simplifier::defeq_canonize_args_step(expr const & e) {
-    buffer<expr> args;
-    bool modified = false;
-    expr f        = get_app_args(e, args);
-    fun_info info = get_fun_info(m_tctx, f, args.size());
-    unsigned i    = 0;
-    for (param_info const & pinfo : info.get_params_info()) {
-        lean_assert(i < args.size());
-        expr new_a;
-        if ((m_canonize_instances_fixed_point && pinfo.is_inst_implicit()) || (m_canonize_proofs_fixed_point && pinfo.is_prop())) {
-            new_a = ::lean::defeq_canonize(m_tctx, args[i], m_need_restart);
-            lean_trace(name({"simplifier", "canonize"}),
-                       tout() << "\n" << args[i] << "\n==>\n" << new_a << "\n";);
-            if (new_a != args[i]) {
-                modified = true;
-                args[i] = new_a;
-            }
-        }
-        i++;
-    }
-
-    if (!modified)
-        return e;
-    else
-        return mk_app(f, args);
-}
-
-simp_result simplifier::simplify_operator_of_app(expr const & e) {
-    lean_assert(is_app(e));
-    buffer<expr> args;
-    expr const & f = get_app_args(e, args);
-    simp_result r_f = simplify(f);
-    return congr_funs(r_f, args);
-}
-
-/* Proving */
-optional<expr> simplifier::prove(expr const & goal) {
-    if (!m_prove_fn)
-        return none_expr();
-
-    metavar_context mctx = m_tctx.mctx();
-    expr goal_mvar = mctx.mk_metavar_decl(m_tctx.lctx(), goal);
-    lean_trace(name({"simplifier", "prove"}), tout() << "goal: " << goal_mvar << " : " << goal << "\n";);
-    vm_obj s = to_obj(tactic_state(m_tctx.env(), m_tctx.get_options(), mctx, list<expr>(goal_mvar), goal_mvar));
-    vm_obj prove_fn_result = invoke(*m_prove_fn, s);
-    optional<tactic_state> s_new = is_tactic_success(prove_fn_result);
-    if (s_new) {
-        if (!s_new->mctx().is_assigned(goal_mvar)) {
-            lean_trace(name({"simplifier", "prove"}), tout() << "prove_fn succeeded but did not return a proof\n";);
-            return none_expr();
-        }
-        metavar_context smctx = s_new->mctx();
-        expr proof = smctx.instantiate_mvars(goal_mvar);
-        optional<expr> new_metavar = find(proof, [&](expr const & e, unsigned) {
-                return is_metavar(e) && !static_cast<bool>(m_tctx.mctx().get_metavar_decl(e));
-            });
-        if (new_metavar) {
-            lean_trace(name({"simplifier", "prove"}),
-                       tout() << "prove_fn succeeded but left an unrecognized metavariable of type "
-                       << smctx.get_metavar_decl(*new_metavar)->get_type() << " in proof\n";);
-            return none_expr();
-        }
-        m_tctx.set_mctx(s_new->mctx());
-        lean_trace(name({"simplifier", "prove"}), tout() << "success: " << proof << " : " << m_tctx.infer(proof) << "\n";);
-        return some_expr(proof);
-    } else {
-        lean_trace(name({"simplifier", "prove"}), tout() << "prove_fn failed to prove " << goal << "\n";);
-        return none_expr();
-    }
-}
-
-/* Congruence */
-
-simp_result simplifier::congr_fun_arg(simp_result const & r_f, simp_result const & r_arg) {
-    if (!r_f.has_proof() && !r_arg.has_proof()) return simp_result(mk_app(r_f.get_new(), r_arg.get_new()));
-    else if (!r_f.has_proof()) return congr_arg(r_f.get_new(), r_arg);
-    else if (!r_arg.has_proof()) return congr_fun(r_f, r_arg.get_new());
-    else return congr(r_f, r_arg);
-}
-
-simp_result simplifier::congr(simp_result const & r_f, simp_result const & r_arg) {
-    lean_assert(r_f.has_proof() && r_arg.has_proof());
-    // theorem congr {A B : Type} {f₁ f₂ : A → B} {a₁ a₂ : A} (H₁ : f₁ = f₂) (H₂ : a₁ = a₂) : f₁ a₁ = f₂ a₂
-    expr e  = mk_app(r_f.get_new(), r_arg.get_new());
-    expr pf = mk_congr(m_tctx, r_f.get_proof(), r_arg.get_proof());
-    return simp_result(e, pf);
-}
-
-simp_result simplifier::congr_fun(simp_result const & r_f, expr const & arg) {
-    lean_assert(r_f.has_proof());
-    // theorem congr_fun {A : Type} {B : A → Type} {f g : Π x, B x} (H : f = g) (a : A) : f a = g a
-    expr e  = mk_app(r_f.get_new(), arg);
-    expr pf = mk_congr_fun(m_tctx, r_f.get_proof(), arg);
-    return simp_result(e, pf);
-}
-
-simp_result simplifier::congr_arg(expr const & f, simp_result const & r_arg) {
-    lean_assert(r_arg.has_proof());
-    // theorem congr_arg {A B : Type} {a₁ a₂ : A} (f : A → B) : a₁ = a₂ → f a₁ = f a₂
-    expr e  = mk_app(f, r_arg.get_new());
-    expr pf = mk_congr_arg(m_tctx, f, r_arg.get_proof());
-    return simp_result(e, pf);
-}
-
-/* Note: handles reflexivity */
-simp_result simplifier::congr_funs(simp_result const & r_f, buffer<expr> const & args) {
-    expr e = r_f.get_new();
-    for (unsigned i = 0; i < args.size(); ++i) {
-        e  = mk_app(e, args[i]);
-    }
-    if (!r_f.has_proof())
-        return simp_result(e);
-    expr pf = r_f.get_proof();
-    for (unsigned i = 0; i < args.size(); ++i) {
-        pf = mk_congr_fun(m_tctx, pf, args[i]);
-    }
-    return simp_result(e, pf);
-}
-
-simp_result simplifier::funext(simp_result const & r, expr const & l) {
-    expr e = m_tctx.mk_lambda(l, r.get_new());
-    if (!r.has_proof())
-        return simp_result(e);
-    expr lam_pf = m_tctx.mk_lambda(l, r.get_proof());
-    expr pf = mk_funext(m_tctx, lam_pf);
-    return simp_result(e, pf);
-}
-
-simp_result simplifier::try_congrs(expr const & e) {
-    simp_lemmas_for const * sls = m_slss.find(m_rel);
-    if (!sls) return simp_result(e);
-
-    list<simp_lemma> const * cls = sls->find_congr(e);
-    if (!cls) return simp_result(e);
-
-    for (simp_lemma const & cl : *cls) {
-        simp_result r = try_congr(e, cl);
-        if (r.get_new() != e)
-            return r;
-    }
-    return simp_result(e);
-}
-
-simp_result simplifier::try_congr(expr const & e, simp_lemma const & cl) {
-    tmp_type_context tmp_tctx(m_tctx, cl.get_num_umeta(), cl.get_num_emeta());
-    if (!tmp_tctx.is_def_eq(e, cl.get_lhs()))
-        return simp_result(e);
-
-    lean_simp_trace(tmp_tctx, name({"debug", "simplifier", "try_congruence"}),
-                    tout() << "(" << cl.get_id() << ") " << e << "\n";);
-
-    bool simplified = false;
-
-    buffer<expr> congr_hyps;
-    to_buffer(cl.get_congr_hyps(), congr_hyps);
-
-    buffer<simp_result> congr_hyp_results;
-    buffer<type_context::tmp_locals> factories;
-    buffer<name> relations;
-    for (expr const & m : congr_hyps) {
-        factories.emplace_back(m_tctx);
-        type_context::tmp_locals & local_factory = factories.back();
-        expr m_type = tmp_tctx.instantiate_mvars(tmp_tctx.infer(m));
-
-        while (is_pi(m_type)) {
-            expr d = instantiate_rev(binding_domain(m_type), local_factory.as_buffer().size(), local_factory.as_buffer().data());
-            expr l = local_factory.push_local(binding_name(m_type), d, binding_info(m_type));
-            lean_assert(!has_metavar(l));
-            m_type = binding_body(m_type);
-        }
-        m_type = instantiate_rev(m_type, local_factory.as_buffer().size(), local_factory.as_buffer().data());
-
-        expr h_rel, h_lhs, h_rhs;
-        lean_verify(is_simp_relation(tmp_tctx.env(), m_type, h_rel, h_lhs, h_rhs) && is_constant(h_rel));
-        {
-            relations.push_back(const_name(h_rel));
-            flet<simp_lemmas> set_slss(m_slss, m_contextual ? add_to_slss(m_slss, local_factory.as_buffer()) : m_slss);
-
-            h_lhs = tmp_tctx.instantiate_mvars(h_lhs);
-            /* TODO(Leo, Daniel): the original assertion was !has_metavar(h_lhs).
-               It is incorrect. I got an assertion violation when processing
-               a term containing universe meta-variables. So, I relaxed it to !has_expr_metavar(h_lhs).
-               We should investigate this. Example: what happens if the input expression has
-               regular meta-variables? Perhaps, the right assertion is: h_lhs does *not* have temporary
-               universe and regular meta-variables. */
-            lean_assert(!has_expr_metavar(h_lhs));
-
-            if (m_contextual || m_rel != const_name(h_rel)) {
-                flet<name> set_name(m_rel, const_name(h_rel));
-                freset<simplify_cache> reset_cache(m_cache);
-                congr_hyp_results.emplace_back(simplify(h_lhs));
-            } else {
-                congr_hyp_results.emplace_back(simplify(h_lhs));
-            }
-            simp_result const & r_congr_hyp = congr_hyp_results.back();
-
-            if (r_congr_hyp.has_proof())
-                simplified = true;
-
-            lean_assert(is_meta(h_rhs));
-            buffer<expr> new_val_meta_args;
-            expr new_val_meta = get_app_args(h_rhs, new_val_meta_args);
-            lean_assert(is_metavar(new_val_meta));
-            expr new_val = tmp_tctx.mk_lambda(new_val_meta_args, r_congr_hyp.get_new());
-            tmp_tctx.assign(new_val_meta, new_val);
-        }
-    }
-
-    if (!simplified)
-        return simp_result(e);
-
-    lean_assert(congr_hyps.size() == congr_hyp_results.size());
-    for (unsigned i = 0; i < congr_hyps.size(); ++i) {
-        expr const & pf_meta = congr_hyps[i];
-        simp_result const & r_congr_hyp = congr_hyp_results[i];
-        name const & rel = relations[i];
-        type_context::tmp_locals & local_factory = factories[i];
-        expr hyp = finalize(m_tctx, rel, r_congr_hyp).get_proof();
-        // This is the current bottleneck
-        // Can address somewhat by keeping the proofs as small as possible using macros
-        expr pf = local_factory.mk_lambda(hyp);
-        tmp_tctx.assign(pf_meta, pf);
-    }
-
-    if (!instantiate_emetas(tmp_tctx, cl.get_num_emeta(), cl.get_emetas(), cl.get_instances()))
-        return simp_result(e);
-
-    for (unsigned i = 0; i < cl.get_num_umeta(); i++) {
-        if (!tmp_tctx.is_uassigned(i))
-            return simp_result(e);
-    }
-
-    expr e_s = tmp_tctx.instantiate_mvars(cl.get_rhs());
-    expr pf = tmp_tctx.instantiate_mvars(cl.get_proof());
-
-    simp_result r(e_s, pf);
-
-    lean_simp_trace(tmp_tctx, name({"simplifier", "congruence"}),
-                    tout() << "(" << cl.get_id() << ") "
-                    << "[" << e << " ==> " << e_s << "]\n";);
-
-    return r;
-}
-
-bool simplifier::instantiate_emetas(tmp_type_context & tmp_tctx, unsigned num_emeta, list<expr> const & emetas, list<bool> const & instances) {
-    bool failed = false;
-    unsigned i = num_emeta;
-    for_each2(emetas, instances, [&](expr const & m, bool const & is_instance) {
-            i--;
-            if (failed) return;
-            expr m_type = tmp_tctx.instantiate_mvars(tmp_tctx.infer(m));
-            if (has_metavar(m_type)) {
-                failed = true;
-                return;
-            }
-
-            if (tmp_tctx.is_eassigned(i)) return;
-
-            if (is_instance) {
-                if (auto v = m_tctx.mk_class_instance(m_type)) {
-                    if (!tmp_tctx.is_def_eq(m, *v)) {
-                        lean_simp_trace(tmp_tctx, name({"simplifier", "failure"}),
-                                        tout() << "unable to assign instance for: " << m_type << "\n";);
-                        failed = true;
-                        return;
-                    }
-                } else {
-                    lean_simp_trace(tmp_tctx, name({"simplifier", "failure"}),
-                                    tout() << "unable to synthesize instance for: " << m_type << "\n";);
-                    failed = true;
-                    return;
-                }
-            }
-
-            if (tmp_tctx.is_eassigned(i)) return;
-
-            // Note: m_type has no metavars
-            if (m_tctx.is_prop(m_type)) {
-                if (auto pf = prove(m_type)) {
-                    lean_verify(tmp_tctx.is_def_eq(m, *pf));
-                    return;
-                }
-            }
-
-            lean_simp_trace(tmp_tctx, name({"simplifier", "failure"}),
-                            tout() << "failed to assign: " << m << " : " << m_type << "\n";);
-
-            failed = true;
-            return;
-        });
-
-    return !failed;
-}
-
-optional<simp_result> simplifier::synth_congr(expr const & e) {
-    lean_assert(is_app(e));
-    buffer<expr> args;
-    expr f = get_app_args(e, args);
-    auto congr_lemma = mk_specialized_congr_simp(m_tctx, e);
-    if (!congr_lemma) return optional<simp_result>();
-
-    buffer<simp_result> r_args;
-    buffer<expr>        new_args;
-    bool has_proof = false;
-    bool has_cast = false;
-    bool has_simplified = false;
-
-    unsigned i = 0;
-
-    // First pass, try to simplify all the Eq arguments
-    for (congr_arg_kind const & ckind : congr_lemma->get_arg_kinds()) {
-        switch (ckind) {
-        case congr_arg_kind::HEq:
-            lean_unreachable();
-        case congr_arg_kind::Fixed:
-        case congr_arg_kind::FixedNoParam:
-            new_args.emplace_back(args[i]);
-            break;
-        case congr_arg_kind::Eq:
-            {
-                r_args.emplace_back(simplify(args[i]));
-                simp_result & r_arg = r_args.back();
-                new_args.emplace_back(r_arg.get_new());
-                if (r_arg.has_proof())
-                    has_proof = true;
-                if (r_arg.get_new() != args[i])
-                    has_simplified = true;
-            }
-            break;
-        case congr_arg_kind::Cast:
-            has_cast = true;
-            new_args.emplace_back(args[i]);
-            break;
-        }
-        i++;
-    }
-
-    if (!has_simplified) {
-        simp_result r = simp_result(e);
-        return optional<simp_result>(r);
-    }
-
-    if (!has_proof) {
-        simp_result r = simp_result(mk_app(f, new_args));
-        return optional<simp_result>(r);
-    }
-
-    // We have a proof, so we need to build the congruence lemma
-    expr proof = congr_lemma->get_proof();
-    expr type = congr_lemma->get_type();
-    buffer<expr> subst;
-
-    i = 0;
-    unsigned i_eq = 0;
-    for (congr_arg_kind const & ckind : congr_lemma->get_arg_kinds()) {
-        switch (ckind) {
-        case congr_arg_kind::HEq:
-            lean_unreachable();
-        case congr_arg_kind::Fixed:
-            proof = mk_app(proof, args[i]);
-            subst.push_back(args[i]);
-            type = binding_body(type);
-            break;
-        case congr_arg_kind::FixedNoParam:
-            break;
-        case congr_arg_kind::Eq:
-            proof = mk_app(proof, args[i]);
-            subst.push_back(args[i]);
-            type = binding_body(type);
-            {
-                simp_result r_arg = finalize(m_tctx, m_rel, r_args[i_eq]);
-                proof = mk_app(proof, r_arg.get_new(), r_arg.get_proof());
-                subst.push_back(r_arg.get_new());
-                subst.push_back(r_arg.get_proof());
-            }
-            type = binding_body(binding_body(type));
-            i_eq++;
-            break;
-        case congr_arg_kind::Cast:
-            lean_assert(has_cast);
-            proof = mk_app(proof, args[i]);
-            subst.push_back(args[i]);
-            type = binding_body(type);
-            break;
-        }
-        i++;
-    }
-    lean_assert(is_eq(type));
-    expr rhs   = instantiate_rev(app_arg(type), subst.size(), subst.data());
-    simp_result r(rhs, proof);
-
-    if (has_cast) {
-        r.update(remove_unnecessary_casts(r.get_new()));
-    }
-
-    return optional<simp_result>(r);
-}
-
-expr simplifier::remove_unnecessary_casts(expr const & e) {
-    buffer<expr> args;
-    expr f = get_app_args(e, args);
-    ss_param_infos ss_infos = get_specialized_subsingleton_info(m_tctx, e);
-    int i = -1;
-    bool updated = false;
-    for (ss_param_info const & ss_info : ss_infos) {
-        i++;
-        if (ss_info.is_subsingleton()) {
-            while (is_constant(get_app_fn(args[i]))) {
-                buffer<expr> cast_args;
-                expr f_cast = get_app_args(args[i], cast_args);
-                name n_f = const_name(f_cast);
-                if (n_f == get_eq_rec_name() || n_f == get_eq_drec_name() || n_f == get_eq_nrec_name()) {
-                    lean_assert(cast_args.size() == 6);
-                    expr major_premise = cast_args[5];
-                    expr f_major_premise = get_app_fn(major_premise);
-                    if (is_constant(f_major_premise) && const_name(f_major_premise) == get_eq_refl_name()) {
-                        args[i] = cast_args[3];
-                        updated = true;
-                    } else {
-                        break;
-                    }
-                } else {
-                    break;
-                }
-            }
-        }
-    }
-    if (!updated)
-        return e;
-
-    expr new_e = mk_app(f, args);
-    lean_trace(name({"debug", "simplifier", "remove_casts"}), tout() << e << " ==> " << new_e << "\n";);
-
-    return mk_app(f, args);
-}
-
-simp_result simplify(type_context & tctx, name const & rel, simp_lemmas const & simp_lemmas,
-                     vm_obj const & prove_fn, expr const & e);
-
-vm_obj simp_lemmas_simplify_core(vm_obj const & lemmas, vm_obj const & prove_fn, vm_obj const & rel_name, vm_obj const & e, vm_obj const & s0) {
-    tactic_state const & s   = to_tactic_state(s0);
+/*
+meta constant simplify_core
+  (c : simplify_config)
+  (s : simp_lemmas)
+  (r : name) :
+  expr → tactic (expr × expr)
+*/
+vm_obj tactic_simplify_core(vm_obj const & c, vm_obj const & slss, vm_obj const & rel, vm_obj const & e, vm_obj const & _s) {
+    tactic_state const & s   = to_tactic_state(_s);
     try {
-        type_context tctx    = mk_type_context_for(s, transparency_mode::Reducible);
-        name rel             = to_name(rel_name);
-        expr old_e           = to_expr(e);
-        simp_result result   = simplify(tctx, rel, to_simp_lemmas(lemmas), prove_fn, old_e);
-
-        if (result.get_new() != old_e) {
-            result = finalize(tctx, rel, result);
+        unsigned max_steps; bool contextual, lift_eq, canonize_instances, canonize_proofs, use_axioms;
+        get_simplify_config(c, max_steps, contextual, lift_eq, canonize_instances, canonize_proofs, use_axioms);
+        type_context ctx     = mk_type_context_for(s, transparency_mode::Reducible);
+        simp_result result   = simplify_fn(ctx, to_simp_lemmas(slss), max_steps, contextual, lift_eq,
+                                           canonize_instances, canonize_proofs, use_axioms)(to_name(rel), to_expr(e));
+        if (result.get_new() != to_expr(e)) {
+            result = finalize(ctx, to_name(rel), result);
             return mk_tactic_success(mk_vm_pair(to_obj(result.get_new()), to_obj(result.get_proof())), s);
         } else {
-            return mk_tactic_exception("simp tactic failed to simplify", s);
+            return mk_tactic_exception("simplify tactic failed to simplify", s);
         }
     } catch (exception & e) {
         return mk_tactic_exception(e, s);
     }
 }
 
-/* Setup and teardown */
+static vm_obj ext_simplify_core(vm_obj const & a, vm_obj const & c, simp_lemmas const & slss, vm_obj const & prove,
+                                vm_obj const & pre, vm_obj const & post, name const & r, expr const & e,
+                                tactic_state const & s) {
+    try {
+        unsigned max_steps; bool contextual, lift_eq, canonize_instances, canonize_proofs, use_axioms;
+        get_simplify_config(c, max_steps, contextual, lift_eq, canonize_instances, canonize_proofs, use_axioms);
+        type_context ctx     = mk_type_context_for(s, transparency_mode::Reducible);
+        vm_simplify_fn simplifier(ctx, slss, max_steps, contextual, lift_eq, canonize_instances, canonize_proofs,
+                                  use_axioms, prove, pre, post);
+        pair<vm_obj, simp_result> p = simplifier(a, r, e);
+        if (p.second.get_new() != e) {
+            vm_obj const & a   = p.first;
+            simp_result result = finalize(ctx, r, p.second);
+            return mk_tactic_success(mk_vm_pair(a, mk_vm_pair(to_obj(result.get_new()), to_obj(result.get_proof()))), s);
+        } else {
+            return mk_tactic_exception("simplify tactic failed to simplify", s);
+        }
+    } catch (exception & e) {
+        return mk_tactic_exception(e, s);
+    }
+}
+
+/*
+meta constant ext_simplify_core
+  {A : Type}
+  (a : A)
+  (c : simplify_config)
+  (l : simp_lemmas)
+  (prove : A → tactic A)
+  (pre : A → name → simp_lemmas → option expr → expr → tactic (A × expr × option expr × bool))
+  (post : A → name → simp_lemmas → option expr → expr → tactic (A × expr × option expr × bool))
+  (r : name) :
+  expr → tactic (A × expr × expr)
+*/
+vm_obj tactic_ext_simplify_core(unsigned num, vm_obj const * args) {
+    lean_assert(num == 10);
+    return ext_simplify_core(args[1], args[2], to_simp_lemmas(args[3]), args[4], args[5], args[6],
+                             to_name(args[7]), to_expr(args[8]), to_tactic_state(args[9]));
+}
+
 void initialize_simplify() {
-    register_trace_class("simplifier");
-    register_trace_class(name({"simplifier", "congruence"}));
-    register_trace_class(name({"simplifier", "failure"}));
-    register_trace_class(name({"simplifier", "failed"}));
-    register_trace_class(name({"simplifier", "perm"}));
-    register_trace_class(name({"simplifier", "canonize"}));
-    register_trace_class(name({"simplifier", "context"}));
-    register_trace_class(name({"simplifier", "prove"}));
-    register_trace_class(name({"simplifier", "rewrite"}));
-    register_trace_class(name({"debug", "simplifier", "try_rewrite"}));
-    register_trace_class(name({"debug", "simplifier", "try_congruence"}));
-    register_trace_class(name({"debug", "simplifier", "remove_casts"}));
+    register_trace_class("simplify");
+    register_trace_class(name({"simplify", "failure"}));
+    register_trace_class(name({"simplify", "context"}));
+    register_trace_class(name({"simplify", "canonize"}));
+    register_trace_class(name({"simplify", "congruence"}));
+    register_trace_class(name({"simplify", "rewrite"}));
+    register_trace_class(name({"simplify", "perm"}));
+    register_trace_class(name({"debug", "simplify", "try_rewrite"}));
+    register_trace_class(name({"debug", "simplify", "try_congruence"}));
 
-    g_simplify_prefix                         = new name{"simplify"};
-
-    g_simplify_max_steps                      = new name{*g_simplify_prefix, "max_steps"};
-    g_simplify_contextual                     = new name{*g_simplify_prefix, "contextual"};
-    g_simplify_rewrite                        = new name{*g_simplify_prefix, "rewrite"};
-    g_simplify_lift_eq                        = new name{*g_simplify_prefix, "lift_eq"};
-    g_simplify_canonize_instances_fixed_point = new name{*g_simplify_prefix, "canonize_instances_fixed_point"};
-    g_simplify_canonize_proofs_fixed_point    = new name{*g_simplify_prefix, "canonize_proofs_fixed_point"};
-
-    register_unsigned_option(*g_simplify_max_steps, LEAN_DEFAULT_SIMPLIFY_MAX_STEPS,
-                             "(simplify) max number of (large) steps in simplification");
-    register_bool_option(*g_simplify_contextual, LEAN_DEFAULT_SIMPLIFY_CONTEXTUAL,
-                         "(simplify) use contextual simplification");
-    register_bool_option(*g_simplify_rewrite, LEAN_DEFAULT_SIMPLIFY_REWRITE,
-                         "(simplify) rewrite with simp_lemmas");
-    register_bool_option(*g_simplify_lift_eq, LEAN_DEFAULT_SIMPLIFY_LIFT_EQ,
-                         "(simplify) try simplifying with equality when no progress over other relation");
-    register_bool_option(*g_simplify_canonize_instances_fixed_point, LEAN_DEFAULT_SIMPLIFY_CANONIZE_INSTANCES_FIXED_POINT,
-                         "(simplify) canonize instances, replacing with the smallest seen so far until reaching a fixed point");
-    register_bool_option(*g_simplify_canonize_proofs_fixed_point, LEAN_DEFAULT_SIMPLIFY_CANONIZE_PROOFS_FIXED_POINT,
-                         "(simplify) canonize proofs, replacing with the smallest seen so far until reaching a fixed point. ");
-
-    DECLARE_VM_BUILTIN(name({"simp_lemmas", "simplify_core"}), simp_lemmas_simplify_core);
+    DECLARE_VM_BUILTIN(name({"tactic", "simplify_core"}), tactic_simplify_core);
+    declare_vm_builtin(name({"tactic", "ext_simplify_core"}),
+                       "tactic_ext_simplify_core", 10, tactic_ext_simplify_core);
 }
 
 void finalize_simplify() {
-    delete g_simplify_canonize_instances_fixed_point;
-    delete g_simplify_canonize_proofs_fixed_point;
-    delete g_simplify_lift_eq;
-    delete g_simplify_rewrite;
-    delete g_simplify_contextual;
-    delete g_simplify_max_steps;
-}
-
-/* Entry point */
-simp_result simplify(type_context & tctx, name const & rel, simp_lemmas const & simp_lemmas, vm_obj const & prove_fn, expr const & e) {
-    return simplifier(tctx, tctx, rel, simp_lemmas, optional<vm_obj>(prove_fn))(e);
-}
-
-simp_result simplify(type_context & tctx, name const & rel, simp_lemmas const & simp_lemmas, expr const & e) {
-    return simplifier(tctx, tctx, rel, simp_lemmas, optional<vm_obj>())(e);
-}
-
-simp_result simplify(type_context & tctx, type_context & tctx_whnf, name const & rel, simp_lemmas const & simp_lemmas, vm_obj const & prove_fn, expr const & e) {
-    return simplifier(tctx, tctx_whnf, rel, simp_lemmas, optional<vm_obj>(prove_fn))(e);
-}
-
-simp_result simplify(type_context & tctx, type_context & tctx_whnf, name const & rel, simp_lemmas const & simp_lemmas, expr const & e) {
-    scope_trace_env scope(tctx.env(), tctx);
-    tout() << e << "\n";
-    return simplifier(tctx, tctx_whnf, rel, simp_lemmas, optional<vm_obj>())(e);
-}
-
-optional<expr> prove_eq_by_simp(type_context & tctx, type_context & tctx_whnf, simp_lemmas const & simp_lemmas, expr const & e) {
-    scope_trace_env scope(tctx.env(), tctx);
-    simp_result r = simplify(tctx, tctx_whnf, get_eq_name(), simp_lemmas, e);
-    expr lhs, rhs;
-    tout() << r.get_new() << "\n-------------\n";
-    if (is_eq(r.get_new(), lhs, rhs) && tctx.is_def_eq(lhs, rhs)) {
-        if (r.has_proof()) {
-            return some_expr(mk_app(tctx, get_eq_mpr_name(), r.get_proof(), mk_eq_refl(tctx, lhs)));
-        } else {
-            return some_expr(mk_eq_refl(tctx, lhs));
-        }
-    } else if (is_true(r.get_new())) {
-        if (r.has_proof()) {
-            return some_expr(mk_app(tctx, get_eq_mpr_name(), r.get_proof(), mk_true_intro()));
-        } else {
-            return some_expr(mk_true_intro());
-        }
-    }
-    return none_expr();
 }
 }
