library/init/default.lean
@@ -7,9 +7,9 @@ prelude
 import init.core init.logic
 import init.relation init.nat init.prod init.sum init.combinator
 import init.bool init.unit init.num init.sigma init.setoid init.quot
-import init.funext init.function init.subtype init.classical
+import init.funext init.function init.subtype init.classical init.congr
 import init.monad init.option init.state init.fin init.list init.char init.string init.to_string
 import init.monad_combinators init.set
 import init.timeit init.trace init.unsigned init.ordering init.list_classes init.coe
 import init.wf init.nat_div init.meta init.instances
-import init.sigma_lex init.simplifier init.id_locked init.order init.algebra
+import init.sigma_lex init.id_locked init.order init.algebra
