tests/lean/run/simp1.lean
@@ -6,6 +6,5 @@ lemma bar : g y = z := sorry
 
 open tactic
 
-set_option trace.simplifier.failure true
 example : g (f x y) = z := by simp
 example : g (f x (f x y)) = z := by simp
