tests/lean/run/simplifier_custom_relations.lean
@@ -26,7 +26,7 @@ print [congr] default
 meta definition relsimp_core (e : expr) : tactic (expr × expr) :=
 do S         ← simp_lemmas.mk_default,
    e_type    ← infer_type e >>= whnf,
-   S^.simplify_core failed `rel e
+   simplify_core default_simplify_config S `rel e
 
 example : rel (h (f x)) z :=
 by do e₁ ← to_expr `(h (f x)),
